Computes
  $$ \begin{aligned}
    f(a, b, c, n) &= \sum^{n}_{i=0} \left\lfloor \frac{a \cdot i + b}{m} \right\rfloor \\
  \end{aligned} $$

Furthermore, Let $m = \left\lfloor\frac{an + b}{c}\right\rfloor$:
  $$ \begin{aligned}
    g(a, b, c, n) &= \sum_{i = 0}^{n}i\left\lfloor\frac{ai + b}{c}\right\rfloor \\
    &= \begin{cases}
        \left\lfloor{\frac{a}{c}}\right\rfloor \cdot \frac{n(n + 1)(2n + 1)}{6} + \left\lfloor\frac{b}{c}\right\rfloor \cdot \frac{n(n + 1)}{2} \\ + g(a\text{ mod } c, b\text{ mod } c, c, n), & a \geq c \lor b \geq c \\
      0, & n < 0 \lor a = 0 \\
      \frac{1}{2} \cdot (n(n + 1)m - f(c, c - b - 1, a, m - 1) \\ - h(c, c - b - 1, a, m - 1)), & \text{otherwise}
    \end{cases}
  \end{aligned} $$
  $$ \begin{aligned}
    h(a, b, c, n) &= \sum_{i = 0}^{n}\left\lfloor\frac{ai + b}{c}\right\rfloor^2 \\
    &= \begin{cases}
        \left\lfloor\frac{a}{c}\right\rfloor^2 \cdot \frac{n(n + 1)(2n + 1)}{6} + \left\lfloor\frac{b}{c}\right\rfloor^2 \cdot (n + 1) \\ + \left\lfloor\frac{a}{c}\right\rfloor \cdot \left\lfloor\frac{b}{c}\right\rfloor \cdot n(n + 1) \\ + h(a\text{ mod } c, b\text{ mod } c, c, n) \\ + 2\left\lfloor\frac{a}{c}\right\rfloor \cdot g(a\text{ mod } c, b\text{ mod } c, c, n) \\ + 2\left\lfloor\frac{b}{c}\right\rfloor \cdot f(a\text{ mod } c, b\text{ mod } c, c, n), & a \geq c \lor b \geq c \\
      0, & n < 0 \lor a = 0 \\
      nm(m + 1) - 2g(c, c - b - 1, a, m - 1) \\ - 2f(c, c - b - 1, a, m - 1) - f(a, b, c, n), & \text{otherwise}
    \end{cases}
  \end{aligned} $$
  
  